Introduce value preservation lemma for the DELEG subsystem

Isabelle/Shelley/Address.thy
@@ -4,6 +4,10 @@ theory Address
   imports Main
 begin
 
+text \<open> Credential \<close>
+
+typedecl credential \<comment> \<open>NOTE: Abstract for now\<close>
+
 text \<open> Output address \<close>
 
 typedecl addr \<comment> \<open>NOTE: Abstract for now\<close>
@@ -11,5 +15,9 @@ typedecl addr \<comment> \<open>NOTE: Abstract for now\<close>
 text \<open> Reward account \<close>
 
 typedecl addr_rwd \<comment> \<open>NOTE: Abstract for now\<close>
+
+text \<open> Construct a reward account \<close>
+
+consts addr_rwd :: "credential \<Rightarrow> addr_rwd" \<comment> \<open>NOTE: Abstract for now\<close>
 
 end
