Isabelle/Shelley/Delegation.thy
@@ -1,12 +1,14 @@
 section \<open> Delegation \<close>
 
 theory Delegation
-  imports Main
+  imports Finite_Map_Extras Basic_Types Address
 begin
+
+subsection \<open> Delegation Definitions \<close>
 
 text \<open> Delegation certificate \<close>
 
-typedecl d_cert \<comment> \<open>NOTE: Abstract for now\<close>
+datatype d_cert = DCert_RegKey | DCert_DeregKey \<comment> \<open>NOTE: Incomplete for now\<close>
 
 text \<open> Registered stake credential \<close>
 
@@ -15,5 +17,47 @@ typedecl stake_creds \<comment> \<open>NOTE: Abstract for now\<close>
 text \<open> Registered stake pools \<close>
 
 typedecl stake_pools \<comment> \<open>NOTE: Abstract for now\<close>
+
+text \<open> Certificate witness \<close>
+
+consts cwitness :: "d_cert \<Rightarrow> credential" \<comment> \<open>NOTE: Abstract for now\<close>
+
+text \<open> Registered credential \<close>
+
+consts reg_cred :: "d_cert \<Rightarrow> credential" \<comment> \<open>NOTE: Abstract for now\<close>
+
+subsection \<open> Delegation Transitions \<close>
+
+text \<open> Delegation States \<close>
+
+type_synonym d_state = "(addr_rwd, coin) fmap" \<comment> \<open>NOTE: Only rewards for now\<close>
+
+text \<open> Delegation Environment \<close>
+
+type_synonym d_env = slot \<comment> \<open>NOTE: Only slot for now\<close>
+
+subsection \<open> Delegation Rules \<close>
+
+text \<open> Delegation Inference Rules \<close>
+
+text \<open> NOTE:
+  Although \<open>addr_rwd hk \<notin> dom rewards \<Longleftrightarrow> hk \<notin> dom stkCreds\<close> is a property of the system,
+  it cannot be proven in \<open>DELEG\<close> alone (but possibly in \<open>DELEGS\<close>). So I had either to add an extra
+  precondition \<open>addr_rwd hk \<notin> dom rewards\<close> or use \<open>\<union>\<^sub>\<leftarrow>\<close> instead of \<open>++\<^sub>f\<close> in rule \<open>deleg_reg\<close> since
+  Lemma 15.6 is a property of \<open>DELEG\<close>.
+ \<close>
+
+inductive deleg_sts :: "d_env \<Rightarrow> d_state \<Rightarrow> d_cert \<Rightarrow> d_state \<Rightarrow> bool"
+  (\<open>_ \<turnstile> _ \<rightarrow>\<^bsub>DELEG\<^esub>{_} _\<close> [51, 0, 51] 50)
+  where
+    deleg_reg: "
+      \<Gamma> \<turnstile> rewards \<rightarrow>\<^bsub>DELEG\<^esub>{c} rewards \<union>\<^sub>\<leftarrow> {addr_rwd hk $$:= 0}"
+      if "c = DCert_RegKey"
+      and "hk = reg_cred c"
+  | deleg_dereg: "
+      \<Gamma> \<turnstile> rewards \<rightarrow>\<^bsub>DELEG\<^esub>{c} {addr_rwd hk} \<lhd>/ rewards"
+      if "c = DCert_DeregKey"
+      and "hk = cwitness c"
+      and "rewards $$ (addr_rwd hk) = Some 0"
 
 end
